rocq/SrsaPeriod.v
@@ -20,80 +20,80 @@ Open Scope Z_scope.
     orders and the same gcd is not a proper factor. *)
 
 Theorem period_base3_period :
-  Z.gcd (pin_sqrt1_mixed - 1) pin_N = pin_p /\
-  Problem_Factor pin_N pin_p.
+  Z.gcd (pin187_sqrt1_mixed - 1) pin187_N = pin187_p /\
+  Problem_Factor pin187_N pin187_p.
 Proof.
   split; [vm_compute; reflexivity|].
-  unfold Problem_Factor. split; [lia|]. exists pin_q. reflexivity.
+  unfold Problem_Factor. split; [lia|]. exists pin187_q. reflexivity.
 Qed.
 
 Theorem period_y32_splits :
-  Z.gcd (pin_sqrt1_mixed - 1) pin_N = pin_p /\
-  Problem_Factor pin_N pin_p.
+  Z.gcd (pin187_sqrt1_mixed - 1) pin187_N = pin187_p /\
+  Problem_Factor pin187_N pin187_p.
 Proof.
   split; [vm_compute; reflexivity|].
-  unfold Problem_Factor. split; [lia|]. exists pin_q. reflexivity.
+  unfold Problem_Factor. split; [lia|]. exists pin187_q. reflexivity.
 Qed.
 
 Theorem period_y5_minus_1_splits :
-  Z.gcd (pin_sqrt1_mixed - 1) pin_N = pin_p /\
-  Problem_Factor pin_N pin_p.
+  Z.gcd (pin187_sqrt1_mixed - 1) pin187_N = pin187_p /\
+  Problem_Factor pin187_N pin187_p.
 Proof.
   split; [vm_compute; reflexivity|].
-  unfold Problem_Factor. split; [lia|]. exists pin_q. reflexivity.
+  unfold Problem_Factor. split; [lia|]. exists pin187_q. reflexivity.
 Qed.
 
 Theorem period_y8_minus_1_splits :
-  Z.gcd (pin_sqrt1_mixed + 1) pin_N = pin_q /\
-  Problem_Factor pin_N pin_q.
+  Z.gcd (pin187_sqrt1_mixed + 1) pin187_N = pin187_q /\
+  Problem_Factor pin187_N pin187_q.
 Proof.
   split; [vm_compute; reflexivity|].
-  unfold Problem_Factor. split; [lia|]. exists pin_p. reflexivity.
+  unfold Problem_Factor. split; [lia|]. exists pin187_p. reflexivity.
 Qed.
 
 Theorem period_y10_minus_1_splits :
-  Z.gcd (pin_sqrt1_mixed - 1) pin_N = pin_p /\
-  Problem_Factor pin_N pin_p.
+  Z.gcd (pin187_sqrt1_mixed - 1) pin187_N = pin187_p /\
+  Problem_Factor pin187_N pin187_p.
 Proof.
   split; [vm_compute; reflexivity|].
-  unfold Problem_Factor. split; [lia|]. exists pin_q. reflexivity.
+  unfold Problem_Factor. split; [lia|]. exists pin187_q. reflexivity.
 Qed.
 
 Theorem period_phi8_y_splits :
-  Z.gcd (pin_sqrt1_mixed + 1) pin_N = pin_q /\
-  Problem_Factor pin_N pin_q.
+  Z.gcd (pin187_sqrt1_mixed + 1) pin187_N = pin187_q /\
+  Problem_Factor pin187_N pin187_q.
 Proof.
   split; [vm_compute; reflexivity|].
-  unfold Problem_Factor. split; [lia|]. exists pin_p. reflexivity.
+  unfold Problem_Factor. split; [lia|]. exists pin187_p. reflexivity.
 Qed.
 
 Theorem period_y2_plus_1_gcd :
-  Z.gcd ((powm pin_y 2 pin_N + 1) mod pin_N) pin_N = 1.
+  Z.gcd ((powm pin187_y 2 pin187_N + 1) mod pin187_N) pin187_N = 1.
 Proof. vm_compute. reflexivity. Qed.
 
 Theorem period_phi5_y_splits :
-  Z.gcd (pin_sqrt1_mixed - 1) pin_N = pin_p /\
-  Problem_Factor pin_N pin_p.
+  Z.gcd (pin187_sqrt1_mixed - 1) pin187_N = pin187_p /\
+  Problem_Factor pin187_N pin187_p.
 Proof.
   split; [vm_compute; reflexivity|].
-  unfold Problem_Factor. split; [lia|]. exists pin_q. reflexivity.
+  unfold Problem_Factor. split; [lia|]. exists pin187_q. reflexivity.
 Qed.
 
 Theorem period_x2_minus_1_int :
-  Z.gcd (pin_x * pin_x - 1) pin_N = 1.
+  Z.gcd (pin187_x * pin187_x - 1) pin187_N = 1.
 Proof. vm_compute. reflexivity. Qed.
 
 Theorem period_full_period_no_split :
-  powm pin_y pin_y_ord pin_N = 1 /\
-  Z.gcd (powm pin_y pin_y_ord pin_N - 1) pin_N = pin_N.
+  powm pin187_y pin187_y_ord pin187_N = 1 /\
+  Z.gcd (powm pin187_y pin187_y_ord pin187_N - 1) pin187_N = pin187_N.
 Proof. vm_compute. split; reflexivity. Qed.
 
 Theorem period_miller_on_period2 :
-  Z.gcd (pin_sqrt1_mixed - 1) pin_N = pin_p /\
-  Problem_Factor pin_N pin_p.
+  Z.gcd (pin187_sqrt1_mixed - 1) pin187_N = pin187_p /\
+  Problem_Factor pin187_N pin187_p.
 Proof.
   split; [vm_compute; reflexivity|].
-  unfold Problem_Factor. split; [lia|]. exists pin_q. reflexivity.
+  unfold Problem_Factor. split; [lia|]. exists pin187_q. reflexivity.
 Qed.
 
 Theorem period_local_orders :
@@ -108,11 +108,11 @@ Theorem period_gcd_pminus1_qminus1 :
 Proof. reflexivity. Qed.
 
 Theorem period_public_d5_pohlig :
-  Z.gcd (pin_sqrt1_mixed - 1) pin_N = pin_p /\
-  Problem_Factor pin_N pin_p.
+  Z.gcd (pin187_sqrt1_mixed - 1) pin187_N = pin187_p /\
+  Problem_Factor pin187_N pin187_p.
 Proof.
   split; [vm_compute; reflexivity|].
-  unfold Problem_Factor. split; [lia|]. exists pin_q. reflexivity.
+  unfold Problem_Factor. split; [lia|]. exists pin187_q. reflexivity.
 Qed.
 
 Theorem period_mismatched_local_orders :
@@ -130,76 +130,76 @@ Theorem period_v2_local_orders :
 Proof. split; reflexivity. Qed.
 
 Theorem period_gcd_path_splits :
-  Z.gcd (pin_sqrt1_mixed - 1) pin_N = pin_p /\
-  Problem_Factor pin_N pin_p.
+  Z.gcd (pin187_sqrt1_mixed - 1) pin187_N = pin187_p /\
+  Problem_Factor pin187_N pin187_p.
 Proof.
   split; [vm_compute; reflexivity|].
-  unfold Problem_Factor. split; [lia|]. exists pin_q. reflexivity.
+  unfold Problem_Factor. split; [lia|]. exists pin187_q. reflexivity.
 Qed.
 
 Theorem period_exp_path_leftover :
-  powm pin_y pin_d pin_N = pin_x /\
-  srsa_residual_leaf pin_N pin_lam pin_y pin_x pin_e.
+  powm pin187_y pin187_d pin187_N = pin187_x /\
+  srsa_residual_leaf pin187_N pin187_lam pin187_y pin187_x pin187_e.
 Proof.
   split; [vm_compute; reflexivity|].
-  apply srsa_residual_pin.
+  apply srsa_residual_pin187.
 Qed.
 
 Theorem period_eq_order_40 :
-  powm pin_y pin_y_ord pin_N = 1 /\
-  powm pin_y 20 pin_N <> 1.
+  powm pin187_y pin187_y_ord pin187_N = 1 /\
+  powm pin187_y 20 pin187_N <> 1.
 Proof. vm_compute. split; [reflexivity | discriminate]. Qed.
 
 Theorem period_eq_not_8 :
-  powm pin_y 8 pin_N <> 1.
+  powm pin187_y 8 pin187_N <> 1.
 Proof. vm_compute. discriminate. Qed.
 
 Theorem period_eq_not_5 :
-  powm pin_y 5 pin_N <> 1.
+  powm pin187_y 5 pin187_N <> 1.
 Proof. vm_compute. discriminate. Qed.
 
 Theorem period_eq_y40 :
-  powm pin_y pin_y_ord pin_N = 1.
+  powm pin187_y pin187_y_ord pin187_N = 1.
 Proof. vm_compute. reflexivity. Qed.
 
 Theorem period_eq_y20 :
-  powm pin_y 20 pin_N <> 1.
+  powm pin187_y 20 pin187_N <> 1.
 Proof. vm_compute. discriminate. Qed.
 
 Theorem period_eq_y8 :
-  powm pin_y 8 pin_N <> 1.
+  powm pin187_y 8 pin187_N <> 1.
 Proof. vm_compute. discriminate. Qed.
 
 Theorem period_eq_y5 :
-  powm pin_y 5 pin_N <> 1.
+  powm pin187_y 5 pin187_N <> 1.
 Proof. vm_compute. discriminate. Qed.
 
 Theorem period_gcd_y5_splits :
-  Z.gcd (pin_sqrt1_mixed - 1) pin_N = pin_p /\
-  Problem_Factor pin_N pin_p.
+  Z.gcd (pin187_sqrt1_mixed - 1) pin187_N = pin187_p /\
+  Problem_Factor pin187_N pin187_p.
 Proof.
   split; [vm_compute; reflexivity|].
-  unfold Problem_Factor. split; [lia|]. exists pin_q. reflexivity.
+  unfold Problem_Factor. split; [lia|]. exists pin187_q. reflexivity.
 Qed.
 
 Theorem period_gcd_y8_splits :
-  Z.gcd (pin_sqrt1_mixed + 1) pin_N = pin_q /\
-  Problem_Factor pin_N pin_q.
+  Z.gcd (pin187_sqrt1_mixed + 1) pin187_N = pin187_q /\
+  Problem_Factor pin187_N pin187_q.
 Proof.
   split; [vm_compute; reflexivity|].
-  unfold Problem_Factor. split; [lia|]. exists pin_p. reflexivity.
+  unfold Problem_Factor. split; [lia|]. exists pin187_p. reflexivity.
 Qed.
 
 Theorem period_gcd_full_period :
-  Z.gcd (powm pin_y pin_y_ord pin_N - 1) pin_N = pin_N.
+  Z.gcd (powm pin187_y pin187_y_ord pin187_N - 1) pin187_N = pin187_N.
 Proof. vm_compute. reflexivity. Qed.
 
 Theorem period_after_ord_invert :
-  powm pin_y pin_d pin_N = pin_x /\
-  srsa_residual_leaf pin_N pin_lam pin_y pin_x pin_e.
+  powm pin187_y pin187_d pin187_N = pin187_x /\
+  srsa_residual_leaf pin187_N pin187_lam pin187_y pin187_x pin187_e.
 Proof.
   split; [vm_compute; reflexivity|].
-  apply srsa_residual_pin.
+  apply srsa_residual_pin187.
 Qed.
 
 Theorem period_v2_ord_p :
@@ -221,85 +221,85 @@ Theorem period_v2_lam_bigger :
 Proof. split; reflexivity. Qed.
 
 Theorem period_x5_minus_1_splits :
-  Z.gcd (pin_sqrt1_mixed - 1) pin_N = pin_p /\
-  Problem_Factor pin_N pin_p.
+  Z.gcd (pin187_sqrt1_mixed - 1) pin187_N = pin187_p /\
+  Problem_Factor pin187_N pin187_p.
 Proof.
   split; [vm_compute; reflexivity|].
-  unfold Problem_Factor. split; [lia|]. exists pin_q. reflexivity.
+  unfold Problem_Factor. split; [lia|]. exists pin187_q. reflexivity.
 Qed.
 
 Theorem period_x8_minus_1_splits :
-  Z.gcd (pin_sqrt1_mixed + 1) pin_N = pin_q /\
-  Problem_Factor pin_N pin_q.
+  Z.gcd (pin187_sqrt1_mixed + 1) pin187_N = pin187_q /\
+  Problem_Factor pin187_N pin187_q.
 Proof.
   split; [vm_compute; reflexivity|].
-  unfold Problem_Factor. split; [lia|]. exists pin_p. reflexivity.
+  unfold Problem_Factor. split; [lia|]. exists pin187_p. reflexivity.
 Qed.
 
 Theorem period_x10_minus_1_splits :
-  Z.gcd (pin_sqrt1_mixed - 1) pin_N = pin_p /\
-  Problem_Factor pin_N pin_p.
+  Z.gcd (pin187_sqrt1_mixed - 1) pin187_N = pin187_p /\
+  Problem_Factor pin187_N pin187_p.
 Proof.
   split; [vm_compute; reflexivity|].
-  unfold Problem_Factor. split; [lia|]. exists pin_q. reflexivity.
+  unfold Problem_Factor. split; [lia|]. exists pin187_q. reflexivity.
 Qed.
 
 Theorem period_x16_minus_1_splits :
-  Z.gcd (pin_sqrt1_mixed + 1) pin_N = pin_q /\
-  Problem_Factor pin_N pin_q.
+  Z.gcd (pin187_sqrt1_mixed + 1) pin187_N = pin187_q /\
+  Problem_Factor pin187_N pin187_q.
 Proof.
   split; [vm_compute; reflexivity|].
-  unfold Problem_Factor. split; [lia|]. exists pin_p. reflexivity.
+  unfold Problem_Factor. split; [lia|]. exists pin187_p. reflexivity.
 Qed.
 
 Theorem period_x4_minus_1 :
-  Z.gcd (powm pin_x 4 pin_N - 1) pin_N = 1.
+  Z.gcd (powm pin187_x 4 pin187_N - 1) pin187_N = 1.
 Proof. vm_compute. reflexivity. Qed.
 
 Theorem period_x2_minus_1 :
-  Z.gcd (powm pin_x 2 pin_N - 1) pin_N = 1.
+  Z.gcd (powm pin187_x 2 pin187_N - 1) pin187_N = 1.
 Proof. vm_compute. reflexivity. Qed.
 
 Theorem period_same_oracle :
-  Z.gcd (pin_sqrt1_mixed - 1) pin_N = pin_p.
+  Z.gcd (pin187_sqrt1_mixed - 1) pin187_N = pin187_p.
 Proof. vm_compute. reflexivity. Qed.
 
 Theorem period_ten_order_16 :
-  powm 2 pin_ord2_q pin_q = 1 /\
-  powm 2 (pin_ord2_q / 2) pin_q <> 1.
+  powm 2 pin187_ord2_q pin187_q = 1 /\
+  powm 2 (pin187_ord2_q / 2) pin187_q <> 1.
 Proof. vm_compute. split; [reflexivity | discriminate]. Qed.
 
 Theorem period_ten_pow8_miller :
-  powm pin_sqrt1_mixed 2 pin_N = 1.
+  powm pin187_sqrt1_mixed 2 pin187_N = 1.
 Proof. vm_compute. reflexivity. Qed.
 
 Theorem period_ten_pow8_splits :
-  Z.gcd (pin_sqrt1_mixed - 1) pin_N = pin_p /\
-  Problem_Factor pin_N pin_p.
+  Z.gcd (pin187_sqrt1_mixed - 1) pin187_N = pin187_p /\
+  Problem_Factor pin187_N pin187_p.
 Proof.
   split; [vm_compute; reflexivity|].
-  unfold Problem_Factor. split; [lia|]. exists pin_q. reflexivity.
+  unfold Problem_Factor. split; [lia|]. exists pin187_q. reflexivity.
 Qed.
 
 Theorem period_ten_pow16 :
-  powm 10 16 pin_N = 1.
+  powm 10 16 pin187_N = 1.
 Proof. vm_compute. reflexivity. Qed.
 
 Theorem period_21_order_4 :
-  powm pin_sqrt1_mixed 2 pin_N = 1.
+  powm pin187_sqrt1_mixed 2 pin187_N = 1.
 Proof. vm_compute. reflexivity. Qed.
 
 Theorem period_21_sq_splits :
-  Z.gcd (pin_sqrt1_mixed - 1) pin_N = pin_p /\
-  Problem_Factor pin_N pin_p.
+  Z.gcd (pin187_sqrt1_mixed - 1) pin187_N = pin187_p /\
+  Problem_Factor pin187_N pin187_p.
 Proof.
   split; [vm_compute; reflexivity|].
-  unfold Problem_Factor. split; [lia|]. exists pin_q. reflexivity.
+  unfold Problem_Factor. split; [lia|]. exists pin187_q. reflexivity.
 Qed.
 
 Theorem period_89_order_4 :
-  powm pin_y 10 pin_N = 89 /\
-  powm 89 4 pin_N = 1.
+  powm pin187_y 10 pin187_N = 89 /\
+  powm 89 4 pin187_N = 1.
 Proof. vm_compute. split; reflexivity. Qed.
 
 Theorem period_77_pminus1 :
@@ -332,76 +332,76 @@ Theorem period_77_ord2_is_lam :
 Proof. split; [vm_compute; reflexivity | vm_compute; reflexivity]. Qed.
 
 Theorem period_two_subgroups_split :
-  Z.gcd (pin_sqrt1_mixed + 1) pin_N = pin_q /\
-  Problem_Factor pin_N pin_q.
+  Z.gcd (pin187_sqrt1_mixed + 1) pin187_N = pin187_q /\
+  Problem_Factor pin187_N pin187_q.
 Proof.
   split; [vm_compute; reflexivity|].
-  unfold Problem_Factor. split; [lia|]. exists pin_p. reflexivity.
+  unfold Problem_Factor. split; [lia|]. exists pin187_p. reflexivity.
 Qed.
 
 Theorem period_three_pohlig_5 :
-  Z.gcd (pin_sqrt1_mixed - 1) pin_N = pin_p /\
-  Problem_Factor pin_N pin_p.
+  Z.gcd (pin187_sqrt1_mixed - 1) pin187_N = pin187_p /\
+  Problem_Factor pin187_N pin187_p.
 Proof.
   split; [vm_compute; reflexivity|].
-  unfold Problem_Factor. split; [lia|]. exists pin_q. reflexivity.
+  unfold Problem_Factor. split; [lia|]. exists pin187_q. reflexivity.
 Qed.
 
 Theorem period_three_pohlig_16 :
-  Z.gcd (pin_sqrt1_mixed + 1) pin_N = pin_q /\
-  Problem_Factor pin_N pin_q.
+  Z.gcd (pin187_sqrt1_mixed + 1) pin187_N = pin187_q /\
+  Problem_Factor pin187_N pin187_q.
 Proof.
   split; [vm_compute; reflexivity|].
-  unfold Problem_Factor. split; [lia|]. exists pin_p. reflexivity.
+  unfold Problem_Factor. split; [lia|]. exists pin187_p. reflexivity.
 Qed.
 
 Theorem period_three_pow8_no_split :
-  Z.gcd (powm pin_g 8 pin_N - 1) pin_N = 1.
+  Z.gcd (powm pin187_g 8 pin187_N - 1) pin187_N = 1.
 Proof. vm_compute. reflexivity. Qed.
 
 Theorem period_cbrt2_cbrt36_split :
-  Z.gcd (pin_sqrt1_mixed + 1) pin_N = pin_q /\
-  Problem_Factor pin_N pin_q.
+  Z.gcd (pin187_sqrt1_mixed + 1) pin187_N = pin187_q /\
+  Problem_Factor pin187_N pin187_q.
 Proof.
   split; [vm_compute; reflexivity|].
-  unfold Problem_Factor. split; [lia|]. exists pin_p. reflexivity.
+  unfold Problem_Factor. split; [lia|]. exists pin187_p. reflexivity.
 Qed.
 
 Theorem period_cbrt3_cbrt36_split :
-  Z.gcd (pin_sqrt1_mixed - 1) pin_N = pin_p /\
-  Problem_Factor pin_N pin_p.
+  Z.gcd (pin187_sqrt1_mixed - 1) pin187_N = pin187_p /\
+  Problem_Factor pin187_N pin187_p.
 Proof.
   split; [vm_compute; reflexivity|].
-  unfold Problem_Factor. split; [lia|]. exists pin_q. reflexivity.
+  unfold Problem_Factor. split; [lia|]. exists pin187_q. reflexivity.
 Qed.
 
 Theorem period_cbrt3_cbrt2 :
-  Z.gcd (75 - 161) pin_N = 1.
+  Z.gcd (75 - 161) pin187_N = 1.
 Proof. vm_compute. reflexivity. Qed.
 
 Theorem period_five_max_order :
-  powm 5 pin_lam pin_N = 1 /\
-  powm 5 pin_y_ord pin_N <> 1.
+  powm 5 pin187_lam pin187_N = 1 /\
+  powm 5 pin187_y_ord pin187_N <> 1.
 Proof. vm_compute. split; [reflexivity | discriminate]. Qed.
 
 Theorem period_five_pohlig_5 :
-  Z.gcd (pin_sqrt1_mixed - 1) pin_N = pin_p /\
-  Problem_Factor pin_N pin_p.
+  Z.gcd (pin187_sqrt1_mixed - 1) pin187_N = pin187_p /\
+  Problem_Factor pin187_N pin187_p.
 Proof.
   split; [vm_compute; reflexivity|].
-  unfold Problem_Factor. split; [lia|]. exists pin_q. reflexivity.
+  unfold Problem_Factor. split; [lia|]. exists pin187_q. reflexivity.
 Qed.
 
 Theorem period_five_pohlig_16 :
-  Z.gcd (pin_sqrt1_mixed + 1) pin_N = pin_q /\
-  Problem_Factor pin_N pin_q.
+  Z.gcd (pin187_sqrt1_mixed + 1) pin187_N = pin187_q /\
+  Problem_Factor pin187_N pin187_q.
 Proof.
   split; [vm_compute; reflexivity|].
-  unfold Problem_Factor. split; [lia|]. exists pin_p. reflexivity.
+  unfold Problem_Factor. split; [lia|]. exists pin187_p. reflexivity.
 Qed.
 
 Theorem period_ord16_to_miller :
-  powm 10 8 pin_N = pin_sqrt1_mixed.
+  powm 10 8 pin187_N = pin187_sqrt1_mixed.
 Proof. vm_compute. reflexivity. Qed.
 
 Theorem period_77_51_is_2_pow7 :
@@ -512,24 +512,24 @@ Theorem period_ord_ndiv_Nminus1 :
 Proof. repeat split; reflexivity. Qed.
 
 Theorem period_Nminus1_divisors_no_split :
-  Z.gcd (powm pin_y 2 pin_N - 1) pin_N = 1 /\
-  Z.gcd (powm pin_y pin_e pin_N - 1) pin_N = 1 /\
-  Z.gcd (powm pin_y 6 pin_N - 1) pin_N = 1 /\
-  Z.gcd (powm pin_y 31 pin_N - 1) pin_N = 1 /\
-  Z.gcd (powm pin_y 62 pin_N - 1) pin_N = 1 /\
-  Z.gcd (powm pin_y 93 pin_N - 1) pin_N = 1.
+  Z.gcd (powm pin187_y 2 pin187_N - 1) pin187_N = 1 /\
+  Z.gcd (powm pin187_y pin187_e pin187_N - 1) pin187_N = 1 /\
+  Z.gcd (powm pin187_y 6 pin187_N - 1) pin187_N = 1 /\
+  Z.gcd (powm pin187_y 31 pin187_N - 1) pin187_N = 1 /\
+  Z.gcd (powm pin187_y 62 pin187_N - 1) pin187_N = 1 /\
+  Z.gcd (powm pin187_y 93 pin187_N - 1) pin187_N = 1.
 Proof. vm_compute. repeat split; reflexivity. Qed.
 
 Theorem period_y_Nminus1_no_annihilator :
-  powm pin_y (pin_N - 1) pin_N = 157 /\
+  powm pin187_y (pin187_N - 1) pin187_N = 157 /\
   157 <> 1 /\
-  Z.gcd (157 - 1) pin_N = 1.
+  Z.gcd (157 - 1) pin187_N = 1.
 Proof. vm_compute. repeat split; discriminate. Qed.
 
 Theorem period_x_Nminus1_no_membership :
-  powm pin_x (pin_N - 1) pin_N = 64 /\
+  powm pin187_x (pin187_N - 1) pin187_N = 64 /\
   64 <> 1 /\
-  Z.gcd (64 - 1) pin_N = 1.
+  Z.gcd (64 - 1) pin187_N = 1.
 Proof. vm_compute. repeat split; discriminate. Qed.
 
 Theorem period_Nplus1_factors :
@@ -537,15 +537,15 @@ Theorem period_Nplus1_factors :
 Proof. reflexivity. Qed.
 
 Theorem period_Nplus1_divisors_no_split :
-  Z.gcd (powm pin_y 4 pin_N - 1) pin_N = 1 /\
-  Z.gcd (powm pin_y 47 pin_N - 1) pin_N = 1 /\
-  Z.gcd (powm pin_y 94 pin_N - 1) pin_N = 1.
+  Z.gcd (powm pin187_y 4 pin187_N - 1) pin187_N = 1 /\
+  Z.gcd (powm pin187_y 47 pin187_N - 1) pin187_N = 1 /\
+  Z.gcd (powm pin187_y 94 pin187_N - 1) pin187_N = 1.
 Proof. vm_compute. repeat split; reflexivity. Qed.
 
 Theorem period_y_Nplus1_no_annihilator :
-  powm pin_y (pin_N + 1) pin_N = 16 /\
+  powm pin187_y (pin187_N + 1) pin187_N = 16 /\
   16 <> 1 /\
-  Z.gcd (16 - 1) pin_N = 1.
+  Z.gcd (16 - 1) pin187_N = 1.
 Proof. vm_compute. repeat split; discriminate. Qed.
 
 (** ** Annihilator quality short of [λ]
@@ -561,46 +561,46 @@ Theorem period_lam_v2_odd_part :
 Proof. split; reflexivity. Qed.
 
 Theorem period_M2_no_split :
-  Z.gcd (powm pin_y 2 pin_N - 1) pin_N = 1.
+  Z.gcd (powm pin187_y 2 pin187_N - 1) pin187_N = 1.
 Proof. vm_compute. reflexivity. Qed.
 
 Theorem period_M4_no_split :
-  Z.gcd (powm pin_y 4 pin_N - 1) pin_N = 1.
+  Z.gcd (powm pin187_y 4 pin187_N - 1) pin187_N = 1.
 Proof. vm_compute. reflexivity. Qed.
 
 Theorem period_advice_odd_part_splits :
-  Z.gcd (pin_sqrt1_mixed - 1) pin_N = pin_p /\
-  Problem_Factor pin_N pin_p.
+  Z.gcd (pin187_sqrt1_mixed - 1) pin187_N = pin187_p /\
+  Problem_Factor pin187_N pin187_p.
 Proof.
   split; [vm_compute; reflexivity|].
-  unfold Problem_Factor. split; [lia|]. exists pin_q. reflexivity.
+  unfold Problem_Factor. split; [lia|]. exists pin187_q. reflexivity.
 Qed.
 
 Theorem period_advice_v2_8_splits :
-  Z.gcd (pin_sqrt1_mixed + 1) pin_N = pin_q /\
-  Problem_Factor pin_N pin_q.
+  Z.gcd (pin187_sqrt1_mixed + 1) pin187_N = pin187_q /\
+  Problem_Factor pin187_N pin187_q.
 Proof.
   split; [vm_compute; reflexivity|].
-  unfold Problem_Factor. split; [lia|]. exists pin_p. reflexivity.
+  unfold Problem_Factor. split; [lia|]. exists pin187_p. reflexivity.
 Qed.
 
 Theorem period_advice_v2_16_splits :
-  Z.gcd (pin_sqrt1_mixed + 1) pin_N = pin_q /\
-  Problem_Factor pin_N pin_q.
+  Z.gcd (pin187_sqrt1_mixed + 1) pin187_N = pin187_q /\
+  Problem_Factor pin187_N pin187_q.
 Proof.
   split; [vm_compute; reflexivity|].
-  unfold Problem_Factor. split; [lia|]. exists pin_p. reflexivity.
+  unfold Problem_Factor. split; [lia|]. exists pin187_p. reflexivity.
 Qed.
 
 Theorem period_advice_ord_invert_no_proper :
-  powm pin_y pin_y_ord pin_N = 1 /\
-  Z.gcd (powm pin_y pin_y_ord pin_N - 1) pin_N = pin_N.
+  powm pin187_y pin187_y_ord pin187_N = 1 /\
+  Z.gcd (powm pin187_y pin187_y_ord pin187_N - 1) pin187_N = pin187_N.
 Proof. vm_compute. split; reflexivity. Qed.
 
 Theorem period_advice_lam_miller :
-  Z.gcd (pin_sqrt1_mixed - 1) pin_N = pin_p /\
-  Problem_Factor pin_N pin_p.
+  Z.gcd (pin187_sqrt1_mixed - 1) pin187_N = pin187_p /\
+  Problem_Factor pin187_N pin187_p.
 Proof.
   split; [vm_compute; reflexivity|].
-  unfold Problem_Factor. split; [lia|]. exists pin_q. reflexivity.
+  unfold Problem_Factor. split; [lia|]. exists pin187_q. reflexivity.
 Qed.
