rocq/SrsaWriteX.v
@@ -25,12 +25,12 @@ Fixpoint xmap_fib_iter (n : nat) (a b : Z) : Z :=
   end.
 
 Theorem xmap_odd_monomial :
-  Z.gcd (pin_sqrt1_mixed + 1) pin_N = pin_q.
+  Z.gcd (pin187_sqrt1_mixed + 1) pin187_N = pin187_q.
 Proof. vm_compute. reflexivity. Qed.
 
 Theorem xmap_associate :
-  powm (pin_N - pin_x) pin_e pin_N = 151 /\
-  151 <> pin_y.
+  powm (pin187_N - pin187_x) pin187_e pin187_N = 151 /\
+  151 <> pin187_y.
 Proof. vm_compute. split; [reflexivity | discriminate]. Qed.
 
 Theorem xmap_midpoint :
@@ -43,8 +43,8 @@ Proof.
 Qed.
 
 Theorem xmap_encrypt_as_decrypt :
-  powm pin_y pin_e pin_N = 93 /\
-  93 <> pin_x.
+  powm pin187_y pin187_e pin187_N = 93 /\
+  93 <> pin187_x.
 Proof. vm_compute. split; [reflexivity | discriminate]. Qed.
 
 Theorem xmap_not_coppersmith_small :
@@ -53,14 +53,14 @@ Theorem xmap_not_coppersmith_small :
 Proof. split; [lia|]. intros Hle. lia. Qed.
 
 Theorem xmap_odd_monomial_y5 :
-  powm pin_y 5 pin_N = 100 /\
-  powm 100 pin_e pin_N = 111 /\
-  111 <> pin_y.
+  powm pin187_y 5 pin187_N = 100 /\
+  powm 100 pin187_e pin187_N = 111 /\
+  111 <> pin187_y.
 Proof. vm_compute. repeat split; discriminate. Qed.
 
 Theorem xmap_y_to_the_y :
-  powm pin_y pin_y pin_N = 135 /\
-  135 <> pin_y.
+  powm pin187_y pin187_y pin187_N = 135 /\
+  135 <> pin187_y.
 Proof. vm_compute. split; [reflexivity | discriminate]. Qed.
 
 Theorem xmap_y_to_the_N :
@@ -68,13 +68,13 @@ Theorem xmap_y_to_the_N :
 Proof. apply srsa_residual_pin. Qed.
 
 Theorem xmap_y_to_Nminus1 :
-  powm pin_y (pin_N - 1) pin_N = 157 /\
-  157 <> pin_y.
+  powm pin187_y (pin187_N - 1) pin187_N = 157 /\
+  157 <> pin187_y.
 Proof. vm_compute. split; [reflexivity | discriminate]. Qed.
 
 Theorem xmap_y_to_Nplus1 :
-  powm pin_y (pin_N + 1) pin_N = 16 /\
-  16 <> pin_y.
+  powm pin187_y (pin187_N + 1) pin187_N = 16 /\
+  16 <> pin187_y.
 Proof. vm_compute. split; [reflexivity | discriminate]. Qed.
 
 Theorem xmap_floor_sqrt_y :
@@ -83,64 +83,64 @@ Theorem xmap_floor_sqrt_y :
 Proof. split; reflexivity. Qed.
 
 Theorem xmap_half_y :
-  pin_y / 2 = 18 /\
-  powm 18 pin_e pin_N = 35 /\
-  35 <> pin_y.
+  pin187_y / 2 = 18 /\
+  powm 18 pin187_e pin187_N = 35 /\
+  35 <> pin187_y.
 Proof. vm_compute. repeat split; discriminate. Qed.
 
 Theorem xmap_bitrev_36_is_9 :
-  Z.gcd (pin_sqrt1_mixed - 1) pin_N = pin_p.
+  Z.gcd (pin187_sqrt1_mixed - 1) pin187_N = pin187_p.
 Proof. vm_compute. reflexivity. Qed.
 
 Theorem xmap_triangular :
-  (pin_y * 35 / 2) mod pin_N = 69 /\
-  powm 69 5 pin_N = 1.
+  (pin187_y * 35 / 2) mod pin187_N = 69 /\
+  powm 69 5 pin187_N = 1.
 Proof. vm_compute. split; reflexivity. Qed.
 
 Theorem xmap_nextprime_as_x :
-  powm 37 pin_e pin_N = 163 /\
-  163 <> pin_y.
+  powm 37 pin187_e pin187_N = 163 /\
+  163 <> pin187_y.
 Proof. vm_compute. split; [reflexivity | discriminate]. Qed.
 
 Theorem xmap_fibonacci_y :
-  Z.gcd (pin_sqrt1_mixed + 1) pin_N = pin_q.
+  Z.gcd (pin187_sqrt1_mixed + 1) pin187_N = pin187_q.
 Proof. vm_compute. reflexivity. Qed.
 
 Theorem xmap_exp_base2 :
-  Z.gcd (pin_sqrt1_mixed - 1) pin_N = pin_p.
+  Z.gcd (pin187_sqrt1_mixed - 1) pin187_N = pin187_p.
 Proof. vm_compute. reflexivity. Qed.
 
 Theorem xmap_exp_base3 :
-  powm pin_g pin_y pin_N = 47 /\
-  47 <> pin_y.
+  powm pin187_g pin187_y pin187_N = 47 /\
+  47 <> pin187_y.
 Proof. vm_compute. split; [reflexivity | discriminate]. Qed.
 
 Theorem xmap_phi3_of_y :
-  (pin_y * pin_y + pin_y + 1) mod pin_N = 24 /\
-  24 <> pin_y.
+  (pin187_y * pin187_y + pin187_y + 1) mod pin187_N = 24 /\
+  24 <> pin187_y.
 Proof. vm_compute. split; [reflexivity | discriminate]. Qed.
 
 Theorem xmap_inv_then_cube :
-  Z.gcd (pin_sqrt1_mixed - 1) pin_N = pin_p.
+  Z.gcd (pin187_sqrt1_mixed - 1) pin187_N = pin187_p.
 Proof. vm_compute. reflexivity. Qed.
 
 Theorem xmap_cube_then_inv :
-  Z.gcd (pin_sqrt1_mixed - 1) pin_N = pin_p.
+  Z.gcd (pin187_sqrt1_mixed - 1) pin187_N = pin187_p.
 Proof. vm_compute. reflexivity. Qed.
 
 Theorem xmap_hybrid_crt :
-  crt2 pin_p pin_q 1 pin_y = 155 /\
-  Z.gcd 155 pin_N = 1 /\
-  powm 155 pin_e pin_N = 144 /\
-  144 <> pin_y.
+  crt2 pin187_p pin187_q 1 pin187_y = 155 /\
+  Z.gcd 155 pin187_N = 1 /\
+  powm 155 pin187_e pin187_N = 144 /\
+  144 <> pin187_y.
 Proof. vm_compute. repeat split; discriminate. Qed.
 
 Theorem xmap_mismatched_crt_splits :
-  Z.gcd (pin_sqrt1_mixed - 1) pin_N = pin_p /\
-  Problem_Factor pin_N pin_p.
+  Z.gcd (pin187_sqrt1_mixed - 1) pin187_N = pin187_p /\
+  Problem_Factor pin187_N pin187_p.
 Proof.
   split; [vm_compute; reflexivity|].
-  unfold Problem_Factor. split; [lia|]. exists pin_q. reflexivity.
+  unfold Problem_Factor. split; [lia|]. exists pin187_q. reflexivity.
 Qed.
 
 Theorem xmap_integer_jnt :
@@ -149,169 +149,169 @@ Theorem xmap_integer_jnt :
 Proof. split; reflexivity. Qed.
 
 Theorem xmap_y2_plus_1 :
-  (pin_y * pin_y + 1) mod pin_N = 175 /\
-  175 <> pin_y.
+  (pin187_y * pin187_y + 1) mod pin187_N = 175 /\
+  175 <> pin187_y.
 Proof. vm_compute. split; [reflexivity | discriminate]. Qed.
 
 Theorem xmap_x_eq_Nminus1 :
-  powm (-1) pin_e pin_N = (pin_N - 1) /\
-  (pin_N - 1) <> pin_y.
+  powm (-1) pin187_e pin187_N = (pin187_N - 1) /\
+  (pin187_N - 1) <> pin187_y.
 Proof. vm_compute. split; [reflexivity | discriminate]. Qed.
 
 Theorem xmap_floor_sqrt_N :
-  0 < pin_N.
+  0 < pin187_N.
 Proof. lia. Qed.
 
 Theorem xmap_phi3_of_N :
-  Z.gcd (pin_N * pin_N + pin_N + 1) pin_lam = 1.
+  Z.gcd (pin187_N * pin187_N + pin187_N + 1) pin187_lam = 1.
 Proof. vm_compute. reflexivity. Qed.
 
 Theorem xmap_y7_onesided :
-  Z.gcd (pin_sqrt1_mixed - 1) pin_N = pin_p.
+  Z.gcd (pin187_sqrt1_mixed - 1) pin187_N = pin187_p.
 Proof. vm_compute. reflexivity. Qed.
 
 Theorem xmap_y9_cubes_to_root :
-  powm pin_y 9 pin_N = 70 /\
-  powm 70 pin_e pin_N = pin_x /\
-  pin_x <> pin_y /\
-  Z.gcd (pin_x - pin_y) pin_N = 1.
+  powm pin187_y 9 pin187_N = 70 /\
+  powm 70 pin187_e pin187_N = pin187_x /\
+  pin187_x <> pin187_y /\
+  Z.gcd (pin187_x - pin187_y) pin187_N = 1.
 Proof. vm_compute. repeat split; try discriminate; reflexivity. Qed.
 
 Theorem xmap_y11_onesided :
-  Z.gcd (pin_sqrt1_mixed + 1) pin_N = pin_q.
+  Z.gcd (pin187_sqrt1_mixed + 1) pin187_N = pin187_q.
 Proof. vm_compute. reflexivity. Qed.
 
 Theorem xmap_floor_y_div_3 :
-  pin_y / 3 = 12 /\
-  powm 12 pin_e pin_N = 45 /\
-  45 <> pin_y.
+  pin187_y / 3 = 12 /\
+  powm 12 pin187_e pin187_N = 45 /\
+  45 <> pin187_y.
 Proof. vm_compute. repeat split; discriminate. Qed.
 
 Theorem xmap_floor_N_div_y :
-  pin_N / pin_y = 5 /\
-  powm 5 pin_e pin_N = 125 /\
-  125 <> pin_y.
+  pin187_N / pin187_y = 5 /\
+  powm 5 pin187_e pin187_N = 125 /\
+  125 <> pin187_y.
 Proof. vm_compute. repeat split; discriminate. Qed.
 
 Theorem xmap_three_y_onesided :
-  Z.gcd (pin_sqrt1_mixed - 1) pin_N = pin_p.
+  Z.gcd (pin187_sqrt1_mixed - 1) pin187_N = pin187_p.
 Proof. vm_compute. reflexivity. Qed.
 
 Theorem xmap_y_minus_1 :
-  powm 35 pin_e pin_N = 52 /\
-  52 <> pin_y.
+  powm 35 pin187_e pin187_N = 52 /\
+  52 <> pin187_y.
 Proof. vm_compute. split; [reflexivity | discriminate]. Qed.
 
 Theorem xmap_y_plus_1_as_x :
-  pin_y + 1 = 37 /\
-  powm 37 pin_e pin_N = 163 /\
-  163 <> pin_y.
+  pin187_y + 1 = 37 /\
+  powm 37 pin187_e pin187_N = 163 /\
+  163 <> pin187_y.
 Proof. vm_compute. repeat split; discriminate. Qed.
 
 Theorem xmap_two_y_plus_1 :
-  2 * pin_y + 1 = 73 /\
-  powm 73 pin_e pin_N = 57 /\
-  57 <> pin_y.
+  2 * pin187_y + 1 = 73 /\
+  powm 73 pin187_e pin187_N = 57 /\
+  57 <> pin187_y.
 Proof. vm_compute. repeat split; discriminate. Qed.
 
 Theorem xmap_y2_minus_1 :
-  (pin_y * pin_y - 1) mod pin_N = 173 /\
-  powm 173 pin_e pin_N = 61 /\
-  61 <> pin_y.
+  (pin187_y * pin187_y - 1) mod pin187_N = 173 /\
+  powm 173 pin187_e pin187_N = 61 /\
+  61 <> pin187_y.
 Proof. vm_compute. repeat split; discriminate. Qed.
 
 Theorem xmap_gray_code :
-  Z.lxor pin_y 18 = 54 /\
-  powm 54 pin_e pin_N = 10 /\
-  10 <> pin_y.
+  Z.lxor pin187_y 18 = 54 /\
+  powm 54 pin187_e pin187_N = 10 /\
+  10 <> pin187_y.
 Proof. vm_compute. repeat split; discriminate. Qed.
 
 Theorem xmap_nibble_swap_nonunit :
-  Z.gcd (pin_sqrt1_mixed - 1) pin_N = pin_p /\
-  Problem_Factor pin_N pin_p.
+  Z.gcd (pin187_sqrt1_mixed - 1) pin187_N = pin187_p /\
+  Problem_Factor pin187_N pin187_p.
 Proof.
   split; [vm_compute; reflexivity|].
-  unfold Problem_Factor. split; [lia|]. exists pin_q. reflexivity.
+  unfold Problem_Factor. split; [lia|]. exists pin187_q. reflexivity.
 Qed.
 
 Theorem xmap_popcount_as_x :
-  pin_y = 2 ^ 5 + 2 ^ 2 /\
-  powm 2 pin_e pin_N = 8 /\
-  8 <> pin_y.
+  pin187_y = 2 ^ 5 + 2 ^ 2 /\
+  powm 2 pin187_e pin187_N = 8 /\
+  8 <> pin187_y.
 Proof. vm_compute. repeat split; discriminate. Qed.
 
 Theorem xmap_catalan_C5 :
   252 / 6 = 42 /\
-  powm pin_x pin_e pin_N = pin_y /\
-  srsa_residual_leaf pin_N pin_lam pin_y pin_x pin_e.
+  powm pin187_x pin187_e pin187_N = pin187_y /\
+  srsa_residual_leaf pin187_N pin187_lam pin187_y pin187_x pin187_e.
 Proof.
   split; [reflexivity|].
   split; [vm_compute; reflexivity|].
-  apply srsa_residual_pin.
+  apply srsa_residual_pin187.
 Qed.
 
 Theorem xmap_lucas_L8 :
-  powm 47 pin_e pin_N = 38 /\
-  38 <> pin_y.
+  powm 47 pin187_e pin187_N = 38 /\
+  38 <> pin187_y.
 Proof. vm_compute. split; [reflexivity | discriminate]. Qed.
 
 Theorem xmap_floor_y_three_halves :
-  216 mod pin_N = 29 /\
-  powm 29 pin_e pin_N = 79 /\
-  79 <> pin_y.
+  216 mod pin187_N = 29 /\
+  powm 29 pin187_e pin187_N = 79 /\
+  79 <> pin187_y.
 Proof. vm_compute. repeat split; discriminate. Qed.
 
 Theorem xmap_shift_left_2_onesided :
-  Z.gcd (pin_sqrt1_mixed + 1) pin_N = pin_q.
+  Z.gcd (pin187_sqrt1_mixed + 1) pin187_N = pin187_q.
 Proof. vm_compute. reflexivity. Qed.
 
 Theorem xmap_y_mod_16 :
-  pin_y mod 16 = 4 /\
-  powm 4 pin_e pin_N = 64 /\
-  64 <> pin_y.
+  pin187_y mod 16 = 4 /\
+  powm 4 pin187_e pin187_N = 64 /\
+  64 <> pin187_y.
 Proof. vm_compute. repeat split; discriminate. Qed.
 
 Theorem xmap_eightbit_palindrome :
-  powm pin_y pin_e pin_N = 93 /\
-  93 <> pin_y.
+  powm pin187_y pin187_e pin187_N = 93 /\
+  93 <> pin187_y.
 Proof. vm_compute. split; [reflexivity | discriminate]. Qed.
 
 Theorem xmap_partition_p10 :
-  powm pin_x pin_e pin_N = pin_y /\
-  srsa_residual_leaf pin_N pin_lam pin_y pin_x pin_e.
+  powm pin187_x pin187_e pin187_N = pin187_y /\
+  srsa_residual_leaf pin187_N pin187_lam pin187_y pin187_x pin187_e.
 Proof.
   split; [vm_compute; reflexivity|].
-  apply srsa_residual_pin.
+  apply srsa_residual_pin187.
 Qed.
 
 Theorem xmap_catalan_C6_nonunit :
-  Z.gcd (pin_sqrt1_mixed - 1) pin_N = pin_p /\
-  Problem_Factor pin_N pin_p.
+  Z.gcd (pin187_sqrt1_mixed - 1) pin187_N = pin187_p /\
+  Problem_Factor pin187_N pin187_p.
 Proof.
   split; [vm_compute; reflexivity|].
-  unfold Problem_Factor. split; [lia|]. exists pin_q. reflexivity.
+  unfold Problem_Factor. split; [lia|]. exists pin187_q. reflexivity.
 Qed.
 
 Theorem xmap_y_inv_sq :
-  powm 26 2 pin_N = 115 /\
-  powm 115 pin_e pin_N = 4 /\
-  4 <> pin_y.
+  powm 26 2 pin187_N = 115 /\
+  powm 115 pin187_e pin187_N = 4 /\
+  4 <> pin187_y.
 Proof. vm_compute. repeat split; discriminate. Qed.
 
 Theorem xmap_x_eq_phi :
-  powm pin_phi pin_e pin_N = 139 /\
-  139 <> pin_y.
+  powm pin187_phi pin187_e pin187_N = 139 /\
+  139 <> pin187_y.
 Proof. vm_compute. split; [reflexivity | discriminate]. Qed.
 
 Theorem xmap_x_bitlength_N :
-  powm 8 pin_e pin_N = 138 /\
-  138 <> pin_y.
+  powm 8 pin187_e pin187_N = 138 /\
+  138 <> pin187_y.
 Proof. vm_compute. split; [reflexivity | discriminate]. Qed.
 
 Theorem xmap_nextprime_mod_N :
-  191 mod pin_N = 4 /\
-  powm 4 pin_e pin_N = 64 /\
-  64 <> pin_y.
+  191 mod pin187_N = 4 /\
+  powm 4 pin187_e pin187_N = 64 /\
+  64 <> pin187_y.
 Proof. vm_compute. repeat split; discriminate. Qed.
 
 Theorem xmap_identity_not_root :
@@ -320,11 +320,11 @@ Theorem xmap_identity_not_root :
 Proof. split; [reflexivity | discriminate]. Qed.
 
 Theorem xmap_y35_onesided :
-  Z.gcd (pin_sqrt1_mixed + 1) pin_N = pin_q /\
-  Problem_Factor pin_N pin_q.
+  Z.gcd (pin187_sqrt1_mixed + 1) pin187_N = pin187_q /\
+  Problem_Factor pin187_N pin187_q.
 Proof.
   split; [vm_compute; reflexivity|].
-  unfold Problem_Factor. split; [lia|]. exists pin_p. reflexivity.
+  unfold Problem_Factor. split; [lia|]. exists pin187_p. reflexivity.
 Qed.
 
 Theorem xmap_inv_lam_minus_1 :
@@ -332,21 +332,21 @@ Theorem xmap_inv_lam_minus_1 :
 Proof. apply srsa_residual_pin. Qed.
 
 Theorem xmap_pkcs_pad :
-  (256 + pin_y) mod pin_N = 105 /\
-  powm 105 pin_e pin_N = 95 /\
-  95 <> pin_y.
+  (256 + pin187_y) mod pin187_N = 105 /\
+  powm 105 pin187_e pin187_N = 95 /\
+  95 <> pin187_y.
 Proof. vm_compute. repeat split; discriminate. Qed.
 
 Theorem xmap_sqrt_then_n_nplus1 :
   6 * 6 = 36 /\
   6 * 7 = 42 /\
-  powm pin_x pin_e pin_N = pin_y /\
-  srsa_residual_leaf pin_N pin_lam pin_y pin_x pin_e.
+  powm pin187_x pin187_e pin187_N = pin187_y /\
+  srsa_residual_leaf pin187_N pin187_lam pin187_y pin187_x pin187_e.
 Proof.
   split; [reflexivity|].
   split; [reflexivity|].
   split; [vm_compute; reflexivity|].
-  apply srsa_residual_pin.
+  apply srsa_residual_pin187.
 Qed.
 
 Theorem xmap_integer_sqrt_unit :
@@ -354,11 +354,11 @@ Theorem xmap_integer_sqrt_unit :
 Proof. apply srsa_residual_pin. Qed.
 
 Theorem xmap_binary_encrypt :
-  powm pin_y 2 pin_N = 174 /\
-  powm pin_y pin_e pin_N = 93 /\
-  93 <> pin_x.
+  powm pin187_y 2 pin187_N = 174 /\
+  powm pin187_y pin187_e pin187_N = 93 /\
+  93 <> pin187_x.
 Proof. vm_compute. repeat split; discriminate. Qed.
 
 Theorem xmap_mont_form :
-  (pin_y * 256) mod pin_N = 53.
+  (pin187_y * 256) mod pin187_N = 53.
 Proof. vm_compute. reflexivity. Qed.
